Fixed building of various HOL OpenTheory packages

src/boss/bool_defsScript.sml
@@ -1,23 +1,37 @@
-open HolKernel boolLib lcsymtacs BasicProvers
+open HolKernel boolLib lcsymtacs BasicProvers;
 
 val _ = new_theory "bool_defs";
 
-val LET_def = new_definition("LET_def",mk_eq(mk_var("LET",type_of(lhs(concl LET_DEF))),rhs(concl LET_DEF)))
+val LET_def = new_definition
+  ("LET_def", mk_eq(mk_var("LET",type_of(lhs(concl LET_DEF))),rhs(concl LET_DEF)));
 
-val literal_case_def = new_definition("literal_case_def",mk_eq(mk_var("literal_case",type_of(lhs(concl literal_case_DEF))),rhs(concl literal_case_DEF)))
+val literal_case_def = new_definition
+  ("literal_case_def",
+    mk_eq(mk_var("literal_case",type_of(lhs(concl literal_case_DEF))),
+          rhs(concl literal_case_DEF)));
 
-val IN_def = new_definition("IN_def",mk_eq(mk_var("IN",type_of(lhs(concl IN_DEF))),rhs(concl IN_DEF)))
+val IN_def = new_definition
+  ("IN_def", mk_eq(mk_var("IN",type_of(lhs(concl IN_DEF))),rhs(concl IN_DEF)));
 
-val TYPE_DEFINITION_def = new_definition("TYPE_DEFINITION_def",mk_eq(mk_var("TYPE_DEFINITION",type_of(lhs(concl TYPE_DEFINITION))),rhs(concl TYPE_DEFINITION)))
+val TYPE_DEFINITION_def = new_definition
+  ("TYPE_DEFINITION_def",
+    mk_eq(mk_var("TYPE_DEFINITION",type_of(lhs(concl TYPE_DEFINITION))),
+          rhs(concl TYPE_DEFINITION)));
 
-val LET_thm = PURE_REWRITE_RULE[FUN_EQ_THM]LET_def |> BETA_RULE |> curry save_thm "LET_thm"
-val literal_case_thm = PURE_REWRITE_RULE[FUN_EQ_THM]literal_case_def |> BETA_RULE |> curry save_thm "literal_case_thm"
-val IN_thm = PURE_REWRITE_RULE[FUN_EQ_THM]IN_def |> BETA_RULE |> curry save_thm "IN_thm"
+val LET_thm = PURE_REWRITE_RULE[FUN_EQ_THM]LET_def
+ |> BETA_RULE |> curry save_thm "LET_thm";
 
-val T_iff = mk_thm([],``!t. (T <=> t) <=> t``)
-val F_iff = mk_thm([],``!t. (F <=> t) <=> ~t``)
+val literal_case_thm = PURE_REWRITE_RULE[FUN_EQ_THM]literal_case_def
+ |> BETA_RULE |> curry save_thm "literal_case_thm";
 
-val TYPE_DEFINITION_thm = store_thm("TYPE_DEFINITION_thm",
+val IN_thm = PURE_REWRITE_RULE[FUN_EQ_THM]IN_def
+ |> BETA_RULE |> curry save_thm "IN_thm";
+
+val T_iff = mk_thm([],``!t. (T <=> t) <=> t``);
+val F_iff = mk_thm([],``!t. (F <=> t) <=> ~t``);
+
+val TYPE_DEFINITION_thm = store_thm
+  ("TYPE_DEFINITION_thm",
   ``!P. (?(rep:'b->'a). TYPE_DEFINITION P rep) ==>
          ?(rep:'b->'a) abs. (!a. abs (rep a) = a) /\ !r. P r <=> (rep (abs r) = r)``,
   PURE_REWRITE_TAC[TYPE_DEFINITION_def]
@@ -51,10 +65,10 @@ val TYPE_DEFINITION_thm = store_thm("TYPE_DEFINITION_thm",
   \\ first_x_assum(qspec_then`r`mp_tac)
   \\ PURE_ASM_REWRITE_TAC[F_iff]
   \\ Ho_Rewrite.PURE_REWRITE_TAC[NOT_EXISTS_THM]
-  \\ disch_then(qspec_then`@x. r = rep x`(ACCEPT_TAC o GSYM)))
+  \\ disch_then(qspec_then`@x. r = rep x`(ACCEPT_TAC o GSYM)));
 
-val _ = Parse.hide"ARB"
-val ARB_def = gen_new_specification("ARB_def",ADD_ASSUM``ARB = @x. F`` TRUTH)
-val ARB_thm = save_thm("ARB_thm",REFL``bool_defs$ARB``)
+val _ = Parse.hide "ARB";
+val ARB_def = gen_new_specification("ARB_def",ADD_ASSUM``ARB = @x. F`` TRUTH);
+val ARB_thm = save_thm("ARB_thm",REFL``bool_defs$ARB``);
 
 val _ = export_theory();
